making some progress on bit rev

crypto_examples/index.dfy
@@ -1,7 +1,7 @@
 include "omega.dfy"
 include "../std_lib/src/Collections/Sequences/LittleEndianNat.dfy"
 
-module bin refines LittleEndianNat {
+module bins refines LittleEndianNat {
     function method BASE(): nat
     {
         2
@@ -10,27 +10,80 @@ module bin refines LittleEndianNat {
 
 module rindex {
     import opened Power
+    import opened Seq
 
     import opened omegas
     import opened pows_of_2
-    import opened bin
+    import opened bins
 
     type uint1   =  i: nat | i < 2
 
-    datatype index_raw = index_cons(v: nat, bin: seq<uint1>)
+    datatype index_raw = index_cons(v: nat, bins: seq<uint1>, bound: pow2_t)
 
     predicate valid_index(idx: index_raw)
     {
-        && idx.v < N == Pow(2, L)
-        && idx.bin == FromNatWithLen(idx.v, L)
+        && idx.v < idx.bound.full
+        && |idx.bins| == idx.bound.exp // exp is the number of bits
+        && idx.v == ToNatRight(idx.bins)
     }
 
     type index_t =  i: index_raw | valid_index(i) witness *
 
     function method build_index(v: nat): index_t
-        requires v < N
+        requires v < N;
     {
         nth_root_lemma();
-        index_cons(v, FromNatWithLen(v, L))
+        index_cons(v, FromNatWithLen(v, L), pow2(L))
+    }
+
+    lemma valid_index_correspondence(idx: index_t)
+        requires 1 <= idx.bound.exp 
+        ensures idx.v % 2 == First(idx.bins);
+        ensures idx.v / 2 == ToNatRight(DropFirst(idx.bins));
+    {
+        pow2_basics(idx.bound);
+        var lsb, v' := idx.v % 2, idx.v / 2;
+        var bins' := DropFirst(idx.bins);
+        reveal ToNatRight();
+        assert lsb == First(idx.bins);
+        assert v' == ToNatRight(bins');
+    }
+
+    function method reverse_bits(idx: index_t): (new_idx: index_raw)
+        requires 1 <= idx.bound.exp < N == Pow(2, L);
+        ensures valid_index(new_idx);
+        decreases idx.bound.exp
+    {
+        if idx.bound.exp == 1 then idx
+        else pow2_basics(idx.bound);
+            var lsb, v' := idx.v % 2, idx.v / 2;
+            var bound' := pow2_half(idx.bound);
+            var bins' := DropFirst(idx.bins);
+            valid_index_correspondence(idx);
+            var temp := index_cons(v', bins', bound');
+            var idx' := reverse_bits(temp);
+            valid_index_correspondence(idx');
+            assert idx'.v + lsb * bound'.full == ToNatRight(idx'.bins + [lsb]) by {
+                calc == {
+                    ToNatRight(idx'.bins + [lsb]);
+                    {
+                        LemmaToNatLeftEqToNatRight(idx'.bins + [lsb]);
+                    }
+                    ToNatLeft(idx'.bins + [lsb]);
+                    {
+                        reveal ToNatLeft();
+                    }
+                    ToNatLeft(idx'.bins) + lsb * Pow(2, idx.bound.exp - 1);
+                    ToNatLeft(idx'.bins) + lsb * bound'.full;
+                    {
+                        LemmaToNatLeftEqToNatRight(idx'.bins);
+                    }
+                    idx'.v + lsb * bound'.full;
+                }
+            }
+            assert idx'.v + lsb * bound'.full < idx.bound.full by {
+                LemmaSeqNatBound(idx'.bins + [lsb]);
+            }
+            index_cons(idx'.v + lsb * bound'.full, idx'.bins + [lsb], idx.bound)
     }
 }
